theories/Basics/Typ_Class2.v
@@ -8,6 +8,8 @@ From ITree Require Import
      Basics.CategoryOps
      Basics.CategoryTheory
      Basics.CategoryFunctor
+     Basics.CategoryRelation
+     Basics.HeterogeneousRelations
 .
 
 Import ProperNotations.
@@ -35,6 +37,7 @@ Class typ : Type :=
 Arguments equal {T}: rename.
 Arguments Typ {Ty} _ {equal_PER}.
 Notation "'equalE' T" := (@equal T) (at level 5).
+Notation "A '==' B" := (equalE _ A B) (at level 50).
 (* This coercion allows us to write [(a: T)] to mean [(a : Ty T)] *)
 Coercion Ty  : typ >-> Sortclass.
 (* Coercion Typ : rel >-> typ. *)
@@ -125,6 +128,7 @@ Qed.
  *)
 Definition arr_typ (TA TB: typ) : typ :=
   Typ (fun (f g: TA -> TB) => forall a1 a2, equal a1 a2 -> equal (f a1) (g a2)).
+
 Notation "e ~~> f" := (arr_typ e f) (at level 60).
 
 (* Elements in the arrow [typ] are exactly the functions respecting the equivalences *)
@@ -139,7 +143,6 @@ Proof.
   Fail typeclasses eauto. (* Still no instance with new Typ definition. *)
 Abort.
 
-
 (*
     Typ forms a Category. We are working in a category C, where:
 
@@ -149,20 +152,23 @@ Abort.
 *)
 Section TypCat.
 
-  Definition typ_proper (TA TB : typ) := {f | Proper (equalE TA ==> equalE TB) f}.
+  Definition typ_proper (TA TB : typ) : Type := { f | Proper (equalE TA ==> equalE TB) f}.
+
+  Definition typ_proper_app : forall {a b : typ} (f : typ_proper a b) (x : a), b :=
+    (fun a b f x => (` f) x).
+
+  Notation "A '-=->' B" := (typ_proper A B) (right associativity, at level 70).
+  Notation "f @ x" := (typ_proper_app f x) (at level 40).
 
   Instance eq2_typ_proper : Eq2 typ_proper :=
-    (fun a b tp tp' =>
-       let f := proj1_sig tp in
-       let g := proj1_sig tp' in
-       forall x y, x ∈ a -> y ∈ a -> equalE a x y -> equalE b (f x) (g y)).
+    (fun a b f g => forall x y, equalE a x y -> equalE b (f @ x) (g @ y)).
 
   Lemma id_ok: forall (TA : typ),
       Proper (equalE TA ==> equalE TA) (fun x => x).
   Proof.
     intros.
     repeat red. tauto.
-  Qed.
+  Defined.
 
   Lemma compose: forall (TA TB TC : typ) (f : TA -> TB) (g : TB -> TC)
       (P1: Proper (equalE TA ==> equalE TB) f)
@@ -181,10 +187,9 @@ Section TypCat.
       (fun x : TA => x) (id_ok TA).
 
   Instance cat_typ_proper : Cat typ_proper :=
-    fun (a b c : typ) (TA : typ_proper a b) (TB : typ_proper b c) =>
+    fun (a b c : typ) (TA : a -=-> b) (TB : b -=-> c) =>
     exist (fun f : a -> c => Proper (equalE a ==> equalE c) f)
-      (fun x : a => (` TB) ((` TA) x))
-      (compose a b c (` TA) (` TB) (proj2_sig TA) (proj2_sig TB)).
+      (fun x : a => TB @ (TA @ x)) (compose a b c _ _ (proj2_sig TA) (proj2_sig TB)).
 
   Instance cat_IdL_typ_proper : CatIdL typ_proper.
     repeat intro. destruct f. cbn. apply p. assumption.
@@ -203,13 +208,132 @@ Section TypCat.
     repeat intro.
     destruct x, y, x0, y0. unfold eq2, eq2_typ_proper in H0.
     cbn in H0. unfold eq2, eq2_typ_proper in H. cbn in H. cbn.
-    specialize (H x1 y1 H1 H2 H3).
+    specialize (H x1 y1 H1).
     specialize (H0 (x x1) (x2 y1)).
-    apply H0. 3 : apply H. apply p. apply H1. apply p0. apply H2.
+    apply H0. apply H.
   Defined.
 
   Global Instance category_typ_proper : Category typ_proper.
     constructor; try typeclasses eauto.
   Defined.
 
+
 End TypCat.
+
+
+Notation "A '-=->' B" := (typ_proper A B) (right associativity, at level 70).
+Notation "f @ x" := (typ_proper_app f x) (at level 40).
+
+
+(* Add proper instances to hint database. *)
+Existing Instance eq2_typ_proper.
+Existing Instance cat_typ_proper.
+Existing Instance id_typ_proper.
+
+
+(* Proper instances for typ and typ_proper. ********************************* *)
+
+Lemma Proper_typ_proper_app : forall {a b : typ},
+    Proper (eq2 ==> equalE a ==> equalE b)
+            (@typ_proper_app a b).
+Proof.
+  repeat intro.
+  destruct x, y.
+  cbn in *.
+  specialize (H x0 y0).
+  cbn in H.
+  apply H. unfold contains. etransitivity. apply H0. symmetry.
+  unfold contains. etransitivity. symmetry. apply H0. apply H0.
+Qed.
+
+(* Lemma Proper_typ_proper_app_partial : forall {a b : typ}  *)
+(*     Proper (equalE a ==> equalE b) *)
+(*             (@typ_proper_app a b x). *)
+(* Proof. *)
+(*   repeat intro. *)
+(*   destruct x, y. *)
+(*   cbn in *. *)
+(*   specialize (H x0 y0). *)
+(*   cbn in H. *)
+(*   apply H. unfold contains. etransitivity. apply H0. symmetry. apply H0. *)
+(*   unfold contains. etransitivity. symmetry. apply H0. apply H0. *)
+(*   assumption. *)
+(* Qed. *)
+
+(* Instance Proper_equal_equal (A : typ) : *)
+(*   Proper (equalE A --> equalE A ==> Basics.impl) (equalE A). *)
+(* Proof. *)
+(*   repeat intro. red in H0. *)
+(*   transitivity x0; [ | assumption]. transitivity x; assumption. *)
+(* Qed. *)
+
+Instance Proper_equal (A : typ) :
+  Proper (equalE A ==> equalE A ==> iff) (equalE A).
+Proof.
+  repeat intro. split.
+  - intro. symmetry. etransitivity.
+    symmetry. apply H0. transitivity x; [ symmetry | ]; assumption.
+  - intro. etransitivity. apply H. transitivity y0; [ | symmetry ]; assumption.
+Qed.
+
+(* Instance Proper_equal_partial (A : typ) (a : A) : *)
+(*   Proper (equalE A --> Basics.flip Basics.impl) (equalE A a). *)
+(* Proof. *)
+(*   repeat intro. red in H. transitivity y ; assumption. *)
+(* Qed. *)
+
+Instance Proper_equal_partial (A : typ) (a : A) :
+  Proper (equalE A ==> iff) (equalE A a).
+Proof.
+  repeat intro. split. intro;
+  etransitivity; eassumption.
+  intro; etransitivity; [ | symmetry ]; eassumption.
+Qed.
+
+(* Add proper instances to hint database. *)
+Existing Instance Proper_typ_proper_app.
+Existing Instance Proper_equal.
+Existing Instance Proper_equal_partial.
+
+
+(* Interesting properties about typ_proper *********************************** *)
+
+Instance eq2_PER : forall a b, PER (eq2 (a := a) (b := b)).
+Proof.
+  pose proof fun_PER.
+  unfold eq2, eq2_typ_proper. intros.
+  specialize (H a b (equalE a) _ (equalE b) _).
+  econstructor.
+  - red. repeat intro. destruct x, y. cbn in *. apply H. apply H0. apply H1.
+  - red. repeat intro. destruct x, y. cbn in *. destruct H. eapply PER_Transitive.
+    eassumption. eassumption. assumption.
+Qed.
+
+Global Instance eq2_Reflexive : forall a b, Reflexive (eq2 (a := a) (b := b)).
+Proof.
+  epose proof cat_IdL_typ_proper. unfold CatIdL in H.
+  repeat intro.
+  specialize (H a b x).
+  unfold eq2, eq2_typ_proper in H.
+  rewrite <- H. 2 : symmetry; apply H0. apply H. etransitivity.
+  symmetry. apply H0. apply H0.
+Defined.
+
+Global Instance eq2_Equivalence : forall a b, Equivalence (eq2 (a := a) (b := b)).
+Proof.
+  intros; constructor; typeclasses eauto.
+Defined.
+
+(* Typ_proper also happens to be a typ. *)
+Definition typ_proper_typ a b : typ :=
+  Typ (eq2 (a := a) (b := b)).
+
+Notation "A ~=~> B" := (typ_proper_typ A B) (at level 80).
+
+(* (* Properness property about exponentials *********************************** *) *)
+
+Global Instance arr_PER: forall a b, PER (equalE (a ~~> b)).
+Proof.
+  pose proof fun_PER.
+  cbn. intros. specialize (H a b (equalE a) _ (equalE b) _). eapply H.
+Defined.
