theories/Basics/PropM.v
@@ -1,0 +1,66 @@
+
+From Coq Require Import
+     Program
+     Setoid
+     Morphisms
+     RelationClasses.
+
+Import ProperNotations.
+From ITree Require Import
+     Typ_Class2
+     Basics.CategoryOps
+     Basics.CategoryTheory
+     Basics.CategoryFunctor
+     Basics.CategoryMonad
+.
+
+Import CatNotations.
+Open Scope cat_scope.
+
+Section MonadProp.
+  Program Definition PropM : typ -> typ :=
+    fun (A : typ) =>
+      {|
+        Ty := {p : A -> Prop | Proper (equalE A ==> iff) p};
+        equal :=
+          fun pm1 pm2 =>
+            forall (a : A), ` pm1 a <-> ` pm2 a
+      |}.
+  Next Obligation.
+    split.
+    repeat red. intros x y H a.
+    split. apply H. apply H.
+    repeat red. intros x y z H H0 a.  
+    split. intros. apply H0, H, H1; auto. intros. apply H, H0, H1; auto.
+  Qed.
+
+  Instance PropM_Monad : Monad typ_proper PropM.
+  split.
+  - repeat red. intros A.
+    refine (exist _ (fun (a:A) => (exist _ (fun x => equalE A a x) _)) _).
+    repeat red. cbn. intros x y Heq a_term.
+    rewrite Heq. auto.
+    Unshelve.
+    repeat red. intros.
+    rewrite H.
+    auto.
+  - repeat red. intros A B HK.
+    destruct HK as (K & KProper).
+    refine (exist _ (fun PA: PropM A => (exist _ (fun b: B =>
+            exists a : A, `PA a /\ (proj1_sig (K a)) b) _)) _).
+    (* KS: For some reason the back-tick didn't work here *)
+    repeat red. cbn. intros ma1 ma2 Heq b.
+    split; intros; destruct H; exists x; specialize (Heq x).
+    + rewrite <- Heq. auto.
+    + rewrite Heq. auto.
+    Unshelve.
+    repeat red. intros b1 b2 Heq.
+    split; intros; destruct H; exists x; destruct H; split; auto.
+      * cbn in *. destruct K.
+        (* KS: Coq can't find the necessary Proper instance to
+               rewrite unless K is destructed. *)
+        rewrite <- Heq. auto.
+      * cbn in *; destruct K; rewrite Heq; auto.
+  Qed.
+
+End MonadProp.
